solvers/19.lean
@@ -2,5 +2,11 @@ import ProjectEulerSolutions.P19
 
 open ProjectEulerSolutions.P19
 
+def startDate : ProjectEulerStatements.P19.Date :=
+  ProjectEulerStatements.P19.mkFirstOfMonth 1901 1 (by decide) (by decide)
+
+def endDate : ProjectEulerStatements.P19.Date :=
+  ProjectEulerStatements.P19.mkFirstOfMonth 2000 12 (by decide) (by decide)
+
 def main : IO Unit := do
-  IO.println (solve 0)
+  IO.println (solve startDate endDate)
